WIP for the dispatcher example

example/Dispatcher.thy
@@ -2,25 +2,25 @@ theory Dispatcher
 
 imports
   "../Parse"
-  "../attic/BasicBlocks"
-  "../Hoare/Hoare"
+  "../Hoare/HoareBasicBlocks"
+  "./ToyExamplesBlocks"
 
 begin
 
 definition 
-dispatch1_hash :: "256 word"
+dispatch1_hash :: "32 word"
 where
 "dispatch1_hash == 0x3ecb5edf"
 
 definition 
-dispatch2_hash :: "256 word"
+dispatch2_hash :: "32 word"
 where
 "dispatch2_hash == 0x8cd5b077"
 
 lemmas blocks_simps = build_blocks_def byteListInt_def find_block_def extract_indexes_def build_vertices_def
  aux_basic_block.simps add_address_def block_pt_def
 
-
+value "parse_bytecode ''90''"
 
 value"blocks_list (build_blocks (parse_bytecode ''60606040526000357c0100000000000000000000000000000000000000000000000000000000900463ffffffff1680633ecb5edf1460475780638cd5b07714607b575b600080fd5b3415605157600080fd5b6065600480803590602001909190505060a1565b6040518082815260200191505060405180910390f35b3415608557600080fd5b608b60ad565b6040518082815260200191505060405180910390f35b6000600190505b919050565b6000600290505b905600a165627a7a72305820c9cf1e9d83721f6f9afecea62b7e868d98502ee8556dcaf6abb24acb8bc0d9fb0029''))"
 
@@ -28,24 +28,24 @@ definition insts where
 "insts \<equiv>
 [Stack (PUSH_N [96]), Stack (PUSH_N [64]), Memory MSTORE, Stack (PUSH_N [0]), Stack CALLDATALOAD,
   Stack (PUSH_N [1, 0, 0, 0, 0, 0, 0, 0, 0, 0, 0, 0, 0, 0, 0, 0, 0, 0, 0, 0, 0, 0, 0, 0, 0, 0, 0, 0, 0]),
-  Swap 1, Arith DIV, Stack (PUSH_N [255, 255, 255, 255]), Bits inst_AND, Dup 1,
-  Stack (PUSH_N [62, 203, 94, 223]), Arith inst_EQ, Stack (PUSH_N [71]), Pc JUMPI, Dup 1,
+  Swap 0, Arith DIV, Stack (PUSH_N [255, 255, 255, 255]), Bits inst_AND, Dup 0,
+  Stack (PUSH_N [62, 203, 94, 223]), Arith inst_EQ, Stack (PUSH_N [71]), Pc JUMPI, Dup 0,
   Stack (PUSH_N [140, 213, 176, 119]), Arith inst_EQ, Stack (PUSH_N [123]), Pc JUMPI, Pc JUMPDEST,
-  Stack (PUSH_N [0]), Dup 1, Unknown 253, Pc JUMPDEST, Info CALLVALUE, Arith ISZERO, Stack (PUSH_N [81]),
-  Pc JUMPI, Stack (PUSH_N [0]), Dup 1, Unknown 253, Pc JUMPDEST, Stack (PUSH_N [101]), Stack (PUSH_N [4]),
-  Dup 1, Dup 1, Stack CALLDATALOAD, Swap 1, Stack (PUSH_N [32]), Arith ADD, Swap 1, Swap 2, Swap 1, Stack POP,
-  Stack POP, Stack (PUSH_N [161]), Pc JUMP, Pc JUMPDEST, Stack (PUSH_N [64]), Memory MLOAD, Dup 1, Dup 3,
-  Dup 2, Memory MSTORE, Stack (PUSH_N [32]), Arith ADD, Swap 2, Stack POP, Stack POP, Stack (PUSH_N [64]),
-  Memory MLOAD, Dup 1, Swap 2, Arith SUB, Swap 1, Misc RETURN, Pc JUMPDEST, Info CALLVALUE, Arith ISZERO,
-  Stack (PUSH_N [133]), Pc JUMPI, Stack (PUSH_N [0]), Dup 1, Unknown 253, Pc JUMPDEST, Stack (PUSH_N [139]),
-  Stack (PUSH_N [173]), Pc JUMP, Pc JUMPDEST, Stack (PUSH_N [64]), Memory MLOAD, Dup 1, Dup 3, Dup 2,
-  Memory MSTORE, Stack (PUSH_N [32]), Arith ADD, Swap 2, Stack POP, Stack POP, Stack (PUSH_N [64]),
-  Memory MLOAD, Dup 1, Swap 2, Arith SUB, Swap 1, Misc RETURN, Pc JUMPDEST, Stack (PUSH_N [0]),
-  Stack (PUSH_N [1]), Swap 1, Stack POP, Pc JUMPDEST, Swap 2, Swap 1, Stack POP, Pc JUMP, Pc JUMPDEST,
-  Stack (PUSH_N [0]), Stack (PUSH_N [2]), Swap 1, Stack POP, Pc JUMPDEST, Swap 1, Pc JUMP, Misc STOP, Log LOG1,
-  Stack (PUSH_N [98, 122, 122, 114, 48, 88]), Arith SHA3, Unknown 201, Unknown 207, Unknown 30, Swap 14, Dup 4,
+  Stack (PUSH_N [0]), Dup 0, Unknown 253, Pc JUMPDEST, Info CALLVALUE, Arith ISZERO, Stack (PUSH_N [81]),
+  Pc JUMPI, Stack (PUSH_N [0]), Dup 0, Unknown 253, Pc JUMPDEST, Stack (PUSH_N [101]), Stack (PUSH_N [4]),
+  Dup 0, Dup 0, Stack CALLDATALOAD, Swap 0, Stack (PUSH_N [32]), Arith ADD, Swap 0, Swap 1, Swap 0, Stack POP,
+  Stack POP, Stack (PUSH_N [161]), Pc JUMP, Pc JUMPDEST, Stack (PUSH_N [64]), Memory MLOAD, Dup 0, Dup 2,
+  Dup 1, Memory MSTORE, Stack (PUSH_N [32]), Arith ADD, Swap 1, Stack POP, Stack POP, Stack (PUSH_N [64]),
+  Memory MLOAD, Dup 0, Swap 1, Arith SUB, Swap 0, Misc RETURN, Pc JUMPDEST, Info CALLVALUE, Arith ISZERO,
+  Stack (PUSH_N [133]), Pc JUMPI, Stack (PUSH_N [0]), Dup 0, Unknown 253, Pc JUMPDEST, Stack (PUSH_N [139]),
+  Stack (PUSH_N [173]), Pc JUMP, Pc JUMPDEST, Stack (PUSH_N [64]), Memory MLOAD, Dup 0, Dup 2, Dup 1,
+  Memory MSTORE, Stack (PUSH_N [32]), Arith ADD, Swap 1, Stack POP, Stack POP, Stack (PUSH_N [64]),
+  Memory MLOAD, Dup 0, Swap 1, Arith SUB, Swap 0, Misc RETURN, Pc JUMPDEST, Stack (PUSH_N [0]),
+  Stack (PUSH_N [1]), Swap 0, Stack POP, Pc JUMPDEST, Swap 1, Swap 0, Stack POP, Pc JUMP, Pc JUMPDEST,
+  Stack (PUSH_N [0]), Stack (PUSH_N [2]), Swap 0, Stack POP, Pc JUMPDEST, Swap 0, Pc JUMP, Misc STOP, Log LOG1,
+  Stack (PUSH_N [98, 122, 122, 114, 48, 88]), Arith SHA3, Unknown 201, Unknown 207, Unknown 30, Swap 13, Dup 3,
   Stack (PUSH_N [31, 111, 154, 254, 206, 166, 43, 126, 134, 141, 152, 80, 46, 232, 85, 109, 202, 246, 171]),
-  Unknown 178, Unknown 74, Unknown 203, Dup 12, Unknown 192, Unknown 217, Unknown 251, Misc STOP, Unknown 41]"
+  Unknown 178, Unknown 74, Unknown 203, Dup 02, Unknown 192, Unknown 217, Unknown 251, Misc STOP, Unknown 41]"
 
 definition blocks where
 "blocks =
@@ -55,48 +55,48 @@ definition blocks where
             (8, Stack (PUSH_N
                         [1, 0, 0, 0, 0, 0, 0, 0, 0, 0, 0, 0, 0, 0, 0, 0, 0, 0, 0, 0, 0, 0, 0, 0, 0, 0, 0, 0,
                          0])),
-            (38, Swap 1), (39, Arith DIV), (40, Stack (PUSH_N [255, 255, 255, 255])), (45, Bits inst_AND),
-            (46, Dup 1), (47, Stack (PUSH_N [62, 203, 94, 223])), (52, Arith inst_EQ),
+            (38, Swap 0), (39, Arith DIV), (40, Stack (PUSH_N [255, 255, 255, 255])), (45, Bits inst_AND),
+            (46, Dup 0), (47, Stack (PUSH_N [62, 203, 94, 223])), (52, Arith inst_EQ),
             (53, Stack (PUSH_N [71]))],
         Jumpi),
-       (56, [(56, Dup 1), (57, Stack (PUSH_N [140, 213, 176, 119])), (62, Arith inst_EQ),
+       (56, [(56, Dup 0), (57, Stack (PUSH_N [140, 213, 176, 119])), (62, Arith inst_EQ),
              (63, Stack (PUSH_N [123]))],
         Jumpi),
-       (66, [(66, Pc JUMPDEST), (67, Stack (PUSH_N [0])), (69, Dup 1), (70, Unknown 253)], Next),
+       (66, [(66, Pc JUMPDEST), (67, Stack (PUSH_N [0])), (69, Dup 0), (70, Unknown 253)], Next),
        (71, [(71, Pc JUMPDEST), (72, Info CALLVALUE), (73, Arith ISZERO), (74, Stack (PUSH_N [81]))], Jumpi),
-       (77, [(77, Stack (PUSH_N [0])), (79, Dup 1), (80, Unknown 253)], Next),
-       (81, [(81, Pc JUMPDEST), (82, Stack (PUSH_N [101])), (84, Stack (PUSH_N [4])), (86, Dup 1), (87, Dup 1),
-             (88, Stack CALLDATALOAD), (89, Swap 1), (90, Stack (PUSH_N [32])), (92, Arith ADD), (93, Swap 1),
-             (94, Swap 2), (95, Swap 1), (96, Stack POP), (97, Stack POP), (98, Stack (PUSH_N [161]))],
+       (77, [(77, Stack (PUSH_N [0])), (79, Dup 0), (80, Unknown 253)], Next),
+       (81, [(81, Pc JUMPDEST), (82, Stack (PUSH_N [101])), (84, Stack (PUSH_N [4])), (86, Dup 0), (87, Dup 0),
+             (88, Stack CALLDATALOAD), (89, Swap 0), (90, Stack (PUSH_N [32])), (92, Arith ADD), (93, Swap 0),
+             (94, Swap 1), (95, Swap 0), (96, Stack POP), (97, Stack POP), (98, Stack (PUSH_N [161]))],
         Jump),
-       (101, [(101, Pc JUMPDEST), (102, Stack (PUSH_N [64])), (104, Memory MLOAD), (105, Dup 1), (106, Dup 3),
-              (107, Dup 2), (108, Memory MSTORE), (109, Stack (PUSH_N [32])), (111, Arith ADD), (112, Swap 2),
+       (101, [(101, Pc JUMPDEST), (102, Stack (PUSH_N [64])), (104, Memory MLOAD), (105, Dup 0), (106, Dup 2),
+              (107, Dup 1), (108, Memory MSTORE), (109, Stack (PUSH_N [32])), (111, Arith ADD), (112, Swap 1),
               (113, Stack POP), (114, Stack POP), (115, Stack (PUSH_N [64])), (117, Memory MLOAD),
-              (118, Dup 1), (119, Swap 2), (120, Arith SUB), (121, Swap 1), (122, Misc RETURN)],
+              (118, Dup 0), (119, Swap 1), (120, Arith SUB), (121, Swap 0), (122, Misc RETURN)],
         No),
        (123, [(123, Pc JUMPDEST), (124, Info CALLVALUE), (125, Arith ISZERO), (126, Stack (PUSH_N [133]))],
         Jumpi),
-       (129, [(129, Stack (PUSH_N [0])), (131, Dup 1), (132, Unknown 253)], Next),
+       (129, [(129, Stack (PUSH_N [0])), (131, Dup 0), (132, Unknown 253)], Next),
        (133, [(133, Pc JUMPDEST), (134, Stack (PUSH_N [139])), (136, Stack (PUSH_N [173]))], Jump),
-       (139, [(139, Pc JUMPDEST), (140, Stack (PUSH_N [64])), (142, Memory MLOAD), (143, Dup 1), (144, Dup 3),
-              (145, Dup 2), (146, Memory MSTORE), (147, Stack (PUSH_N [32])), (149, Arith ADD), (150, Swap 2),
+       (139, [(139, Pc JUMPDEST), (140, Stack (PUSH_N [64])), (142, Memory MLOAD), (143, Dup 0), (144, Dup 2),
+              (145, Dup 1), (146, Memory MSTORE), (147, Stack (PUSH_N [32])), (149, Arith ADD), (150, Swap 1),
               (151, Stack POP), (152, Stack POP), (153, Stack (PUSH_N [64])), (155, Memory MLOAD),
-              (156, Dup 1), (157, Swap 2), (158, Arith SUB), (159, Swap 1), (160, Misc RETURN)],
+              (156, Dup 0), (157, Swap 1), (158, Arith SUB), (159, Swap 0), (160, Misc RETURN)],
         No),
-       (161, [(161, Pc JUMPDEST), (162, Stack (PUSH_N [0])), (164, Stack (PUSH_N [1])), (166, Swap 1),
+       (161, [(161, Pc JUMPDEST), (162, Stack (PUSH_N [0])), (164, Stack (PUSH_N [1])), (166, Swap 0),
               (167, Stack POP)],
         Next),
-       (168, [(168, Pc JUMPDEST), (169, Swap 2), (170, Swap 1), (171, Stack POP)], Jump),
-       (173, [(173, Pc JUMPDEST), (174, Stack (PUSH_N [0])), (176, Stack (PUSH_N [2])), (178, Swap 1),
+       (168, [(168, Pc JUMPDEST), (169, Swap 1), (170, Swap 0), (171, Stack POP)], Jump),
+       (173, [(173, Pc JUMPDEST), (174, Stack (PUSH_N [0])), (176, Stack (PUSH_N [2])), (178, Swap 0),
               (179, Stack POP)],
         Next),
-       (180, [(180, Pc JUMPDEST), (181, Swap 1)], Jump), (183, [(183, Misc STOP)], No),
+       (180, [(180, Pc JUMPDEST), (181, Swap 0)], Jump), (183, [(183, Misc STOP)], No),
        (184, [(184, Log LOG1), (185, Stack (PUSH_N [98, 122, 122, 114, 48, 88])), (192, Arith SHA3),
-              (193, Unknown 201), (194, Unknown 207), (195, Unknown 30), (196, Swap 14), (197, Dup 4),
+              (193, Unknown 201), (194, Unknown 207), (195, Unknown 30), (196, Swap 13), (197, Dup 3),
               (198, Stack (PUSH_N
                             [31, 111, 154, 254, 206, 166, 43, 126, 134, 141, 152, 80, 46, 232, 85, 109, 202,
                              246, 171])),
-              (218, Unknown 178), (219, Unknown 74), (220, Unknown 203), (221, Dup 12), (222, Unknown 192),
+              (218, Unknown 178), (219, Unknown 74), (220, Unknown 203), (221, Dup 02), (222, Unknown 192),
               (223, Unknown 217), (224, Unknown 251), (225, Misc STOP)],
         No),
        (226, [(226, Unknown 41)], Next)],
@@ -106,62 +106,146 @@ definition blocks where
             (8, Stack (PUSH_N
                         [1, 0, 0, 0, 0, 0, 0, 0, 0, 0, 0, 0, 0, 0, 0, 0, 0, 0, 0, 0, 0, 0, 0, 0, 0, 0, 0, 0,
                          0])),
-            (38, Swap 1), (39, Arith DIV), (40, Stack (PUSH_N [255, 255, 255, 255])), (45, Bits inst_AND),
-            (46, Dup 1), (47, Stack (PUSH_N [62, 203, 94, 223])), (52, Arith inst_EQ),
+            (38, Swap 0), (39, Arith DIV), (40, Stack (PUSH_N [255, 255, 255, 255])), (45, Bits inst_AND),
+            (46, Dup 0), (47, Stack (PUSH_N [62, 203, 94, 223])), (52, Arith inst_EQ),
             (53, Stack (PUSH_N [71]))],
         Jumpi),
-       (56, [(56, Dup 1), (57, Stack (PUSH_N [140, 213, 176, 119])), (62, Arith inst_EQ),
+       (56, [(56, Dup 0), (57, Stack (PUSH_N [140, 213, 176, 119])), (62, Arith inst_EQ),
              (63, Stack (PUSH_N [123]))],
         Jumpi),
-       (66, [(66, Pc JUMPDEST), (67, Stack (PUSH_N [0])), (69, Dup 1), (70, Unknown 253)], Next),
+       (66, [(66, Pc JUMPDEST), (67, Stack (PUSH_N [0])), (69, Dup 0), (70, Unknown 253)], Next),
        (71, [(71, Pc JUMPDEST), (72, Info CALLVALUE), (73, Arith ISZERO), (74, Stack (PUSH_N [81]))], Jumpi),
-       (77, [(77, Stack (PUSH_N [0])), (79, Dup 1), (80, Unknown 253)], Next),
-       (81, [(81, Pc JUMPDEST), (82, Stack (PUSH_N [101])), (84, Stack (PUSH_N [4])), (86, Dup 1), (87, Dup 1),
-             (88, Stack CALLDATALOAD), (89, Swap 1), (90, Stack (PUSH_N [32])), (92, Arith ADD), (93, Swap 1),
-             (94, Swap 2), (95, Swap 1), (96, Stack POP), (97, Stack POP), (98, Stack (PUSH_N [161]))],
+       (77, [(77, Stack (PUSH_N [0])), (79, Dup 0), (80, Unknown 253)], Next),
+       (81, [(81, Pc JUMPDEST), (82, Stack (PUSH_N [101])), (84, Stack (PUSH_N [4])), (86, Dup 0), (87, Dup 0),
+             (88, Stack CALLDATALOAD), (89, Swap 0), (90, Stack (PUSH_N [32])), (92, Arith ADD), (93, Swap 0),
+             (94, Swap 1), (95, Swap 0), (96, Stack POP), (97, Stack POP), (98, Stack (PUSH_N [161]))],
         Jump),
-       (101, [(101, Pc JUMPDEST), (102, Stack (PUSH_N [64])), (104, Memory MLOAD), (105, Dup 1), (106, Dup 3),
-              (107, Dup 2), (108, Memory MSTORE), (109, Stack (PUSH_N [32])), (111, Arith ADD), (112, Swap 2),
+       (101, [(101, Pc JUMPDEST), (102, Stack (PUSH_N [64])), (104, Memory MLOAD), (105, Dup 0), (106, Dup 2),
+              (107, Dup 1), (108, Memory MSTORE), (109, Stack (PUSH_N [32])), (111, Arith ADD), (112, Swap 1),
               (113, Stack POP), (114, Stack POP), (115, Stack (PUSH_N [64])), (117, Memory MLOAD),
-              (118, Dup 1), (119, Swap 2), (120, Arith SUB), (121, Swap 1), (122, Misc RETURN)],
+              (118, Dup 0), (119, Swap 1), (120, Arith SUB), (121, Swap 0), (122, Misc RETURN)],
         No),
        (123, [(123, Pc JUMPDEST), (124, Info CALLVALUE), (125, Arith ISZERO), (126, Stack (PUSH_N [133]))],
         Jumpi),
-       (129, [(129, Stack (PUSH_N [0])), (131, Dup 1), (132, Unknown 253)], Next),
+       (129, [(129, Stack (PUSH_N [0])), (131, Dup 0), (132, Unknown 253)], Next),
        (133, [(133, Pc JUMPDEST), (134, Stack (PUSH_N [139])), (136, Stack (PUSH_N [173]))], Jump),
-       (139, [(139, Pc JUMPDEST), (140, Stack (PUSH_N [64])), (142, Memory MLOAD), (143, Dup 1), (144, Dup 3),
-              (145, Dup 2), (146, Memory MSTORE), (147, Stack (PUSH_N [32])), (149, Arith ADD), (150, Swap 2),
+       (139, [(139, Pc JUMPDEST), (140, Stack (PUSH_N [64])), (142, Memory MLOAD), (143, Dup 0), (144, Dup 2),
+              (145, Dup 1), (146, Memory MSTORE), (147, Stack (PUSH_N [32])), (149, Arith ADD), (150, Swap 1),
               (151, Stack POP), (152, Stack POP), (153, Stack (PUSH_N [64])), (155, Memory MLOAD),
-              (156, Dup 1), (157, Swap 2), (158, Arith SUB), (159, Swap 1), (160, Misc RETURN)],
+              (156, Dup 0), (157, Swap 1), (158, Arith SUB), (159, Swap 0), (160, Misc RETURN)],
         No),
-       (161, [(161, Pc JUMPDEST), (162, Stack (PUSH_N [0])), (164, Stack (PUSH_N [1])), (166, Swap 1),
+       (161, [(161, Pc JUMPDEST), (162, Stack (PUSH_N [0])), (164, Stack (PUSH_N [1])), (166, Swap 0),
               (167, Stack POP)],
         Next),
-       (168, [(168, Pc JUMPDEST), (169, Swap 2), (170, Swap 1), (171, Stack POP)], Jump),
-       (173, [(173, Pc JUMPDEST), (174, Stack (PUSH_N [0])), (176, Stack (PUSH_N [2])), (178, Swap 1),
+       (168, [(168, Pc JUMPDEST), (169, Swap 1), (170, Swap 0), (171, Stack POP)], Jump),
+       (173, [(173, Pc JUMPDEST), (174, Stack (PUSH_N [0])), (176, Stack (PUSH_N [2])), (178, Swap 0),
               (179, Stack POP)],
         Next),
-       (180, [(180, Pc JUMPDEST), (181, Swap 1)], Jump), (183, [(183, Misc STOP)], No),
+       (180, [(180, Pc JUMPDEST), (181, Swap 0)], Jump), (183, [(183, Misc STOP)], No),
        (184, [(184, Log LOG1), (185, Stack (PUSH_N [98, 122, 122, 114, 48, 88])), (192, Arith SHA3),
-              (193, Unknown 201), (194, Unknown 207), (195, Unknown 30), (196, Swap 14), (197, Dup 4),
+              (193, Unknown 201), (194, Unknown 207), (195, Unknown 30), (196, Swap 13), (197, Dup 3),
               (198, Stack (PUSH_N
                             [31, 111, 154, 254, 206, 166, 43, 126, 134, 141, 152, 80, 46, 232, 85, 109, 202,
                              246, 171])),
-              (218, Unknown 178), (219, Unknown 74), (220, Unknown 203), (221, Dup 12), (222, Unknown 192),
+              (218, Unknown 178), (219, Unknown 74), (220, Unknown 203), (221, Dup 02), (222, Unknown 192),
               (223, Unknown 217), (224, Unknown 251), (225, Misc STOP)],
         No),
        (226, [(226, Unknown 41)], Next)]\<rparr>"
+context
+notes if_split[ split del ] sep_fun_simps[simp del]
+gas_value_simps[simp add] pure_emp_simps[simp add]
+evm_fun_simps[simp add] sep_lc[simp del] sep_conj_first[simp add]
+pure_false_simps[simp add] iszero_stack_def[simp add]
+begin
 
+lemma aux1:
+"(word_of_int (bin_rcat 8 [62, 203, 94, 223]) ::w256)=
+    word_of_int (bin_rcat 8 [255, 255, 255, 255]) AND
+    (if word_of_int
+         (bin_rcat 8
+           [1, 0, 0, 0, 0, 0, 0, 0, 0, 0, 0, 0, 0, 0, 0, 0, 0, 0, 0,
+            0, 0, 0, 0, 0, 0, 0, 0, 0, 0]) =
+        (0::w256)
+     then word_of_int 0
+     else word_of_int
+           (uint
+             (read_word_from_bytes
+               (unat (word_of_int (bin_rcat 8 [0])))
+               (word_rsplit dispatch1_hash)) div
+            uint
+             (word_of_int
+               (bin_rcat 8
+                 [1, 0, 0, 0, 0, 0, 0, 0, 0, 0, 0, 0, 0, 0, 0, 0, 0,
+                  0, 0, 0, 0, 0, 0, 0, 0, 0, 0, 0, 0])::w256)))"
+apply(split if_splits)
+ apply(simp add: bin_rcat_def bin_cat_def)
+unfolding read_word_from_bytes_def dispatch1_hash_def
+apply simp
+apply (simp add: byte_list_fill_right_def)
+apply (simp add: word_rcat_def bin_rcat_def bin_cat_def  )
+done
+
+method sep_imp_solve =
+clarsimp?;
+(rule conjI),
+  (clarsimp simp add: word_rcat_def)?,
+  (sep_cancel)+,
+  (erule instantiate_emp)?,
+(simp add:M_def Cmem_def bin_rcat_def)?
+
+method sep_imp_solve_sep_cancel_simp =
+(clarsimp),
+(rule conjI),
+  (clarsimp simp add: word_rcat_def)?,
+  (sep_cancel, simp?)+,
+  (erule instantiate_emp)?,
+(simp add:M_def Cmem_def bin_rcat_def)?
+value "word_rsplit (0x3ecb5edf::32 word):: byte list"
 lemma
-"triple_blocks blocks (initial_state ** (data_lst dispatch1_hash) ** sent_value 0) (action (ContractReturn (word_rsplit (1:: w256))))"
-apply (simp add: blocks_def)
-
+"\<exists>r.
+triple 
+  (
+program_counter 0 ** stack_height 0 ** (data_lst 0 (word_rsplit dispatch1_hash)) ** sent_value 0 **
+   memory_usage 0 ** continuing ** gas_pred 3000 ** memory (word_rcat [64::byte]) (word_rcat [x::byte]::256 word))
+  blocks
+  (action (ContractReturn (word_rsplit (1:: w256))) ** r)"
+apply (simp add: blocks_def triple_def)
+apply(rule exI)
+apply(triple_jumpi_vcg)
+    apply(simp add: Cmem_def M_def word_rsplit_def bin_rsplit_def)
+   apply(sep_imp_solve_sep_cancel_simp | sep_imp_solve)+
+  apply(simp add: bin_rcat_def)
+ apply(simp add: aux1)
+ defer
+ apply(simp add: aux1)
+ apply(subst sym[OF aux1])
+ apply(simp add: bin_rcat_def)
+apply((rule blocks_jumpi; (rule refl)?), triple_seq_vcg)
+apply(sep_imp_solve_sep_cancel_simp | sep_imp_solve)+
+apply(simp add: bin_rcat_def)+
+defer 
+apply(simp)
+apply((rule blocks_jump; (rule refl)?), triple_seq_vcg)
+apply(sep_imp_solve_sep_cancel_simp | sep_imp_solve)+
+apply(simp add: bin_rcat_def)+
+apply((rule blocks_next; (rule refl)?), triple_seq_vcg)
+apply(sep_imp_solve_sep_cancel_simp | sep_imp_solve)+
+apply(simp add: bin_rcat_def)+
+apply((rule blocks_jump; (rule refl)?), triple_seq_vcg)
+apply(sep_imp_solve_sep_cancel_simp | sep_imp_solve)
+apply(sep_imp_solve_sep_cancel_simp | sep_imp_solve)
+apply(sep_imp_solve_sep_cancel_simp | sep_imp_solve)
+apply(sep_imp_solve_sep_cancel_simp | sep_imp_solve)
+apply(clarsimp)
+apply(rule conjI)
+apply  (clarsimp simp add: word_rcat_def)?
+apply  (sep_cancel, simp?)+
+apply  (erule instantiate_emp)?
+(simp add:M_def Cmem_def bin_rcat_def)?
+apply(sep_imp_solve_sep_cancel_simp | sep_imp_solve)
+apply(simp add: bin_rcat_def)+
 sorry
-typ "256 word \<Rightarrow> (byte list \<Rightarrow> byte list)"
-lemma
-"triple_blocks blocks (initial_state ** (data_lst dispatch_hash) ** ( if dispatch_hash = dispatch1_hash then (data_lst dispatch_hash) else emp) ** sent_value 0) 
-( if dispatch_hash = dispatch1_hash then action (ContractReturn (word_rsplit (1:: w256))) else ())"
-apply (simp add: blocks_def)
-
-
+value "word_rsplit (0x3ecb5edf::w256):: byte list"
+value "byte_list_fill_right  0 32 ([62, 203, 94, 223]::byte list)"
+end
 end
